Proof of new_or_old

Proof.fst
@@ -1,3 +1,10 @@
+module Proof
+
+open FStar.IO
+open FStar.Printf
+open FStar.List
+open FStar.List.Tot.Base
+
 type english_letters =
   | A
   | B
@@ -25,72 +32,369 @@ type english_letters =
   | X 
   | Y 
   | Z
-  
+
 val alphabet : list english_letters 
 let alphabet = [A;B;C;D;E;F;G;H;I;J;K;M;N;O;P;Q;R;S;T;U;V;W;X;Y;Z]
   
 val text : list english_letters
-let text = [A;B;A;B;X;A;B;Z;A;B;A;B;A;B]
+let text = [E;A;A;A;X;A;B;X;A;A;X;B;A;X;B;A;A;A;B;A;B;B]
 
 val pattern : list english_letters
-let pattern = [Z;A;B;A;B;A;B]
+let pattern = [E;A;A;A;X;E;C;F;C]
 
-val length (#a:Type) (l:list a) : nat
-let rec length l
-  = match l with
-      | [] -> 0
-      | hd :: tl -> 1 + length tl
-
-val alphabet_length : nat
+val alphabet_length : (i:nat{i > 0})
 let alphabet_length = length alphabet
 
-val alphabet_character_index (c:english_letters) (l:list english_letters) (i:int): int
-let rec alphabet_character_index c l i
-  = match l with 
-      | [] -> -1
-      | hd::tl -> if hd = c
-                  then i
-                  else alphabet_character_index c tl (i+1)
-      
-val verify_character_in_pattern (c:english_letters) (l:list english_letters) : bool
-let rec verify_character_in_pattern c l =
-    match l with
-        | [] -> false
-        | hd::tl -> if hd = c
-                    then true
-                    else verify_character_in_pattern c tl
+//equivalent with mem c l 
+// val verify_character_in_pattern (c:english_letters) (l:list english_letters) : bool
+// let rec verify_character_in_pattern c l =
+//     match l with
+//         | [] -> false
+//         | hd::tl -> if hd = c
+//                     then true
+//                     else verify_character_in_pattern c tl
 
-val change_element_in_bc_list (l:list int) (i:int) (j:int) (n:int) : list int
-let rec change_element_in_bc_list l i j n=
-    match l with
-        | [] -> []
-        | hd::tl -> if i = j
-                    then n::change_element_in_bc_list tl (i + 1) j n
-                    else hd::change_element_in_bc_list tl (i + 1) j n
+//equivalent with map (new_or_old) l
+// val change_element_in_bc_list (l:list int) (i:int) (j:int) (n:int) : list int
+// let rec change_element_in_bc_list l i j n=
+//     match l with
+//         | [] -> []
+//         | hd::tl -> if i = j
+//                     then n::change_element_in_bc_list tl (i + 1) j n
+//                     else hd::change_element_in_bc_list tl (i + 1) j n
 
-val create_bc (i:nat{i >= 0}) : list int
-let rec create_bc i 
+let rec create_bc (i:nat) : Tot (list int) (decreases i) 
   =match i with
       | 0 -> []
       | _ -> (-1) :: (create_bc (i-1))
-      
+
+let rec length_create_bc_is_positive (i:nat)
+  : Lemma (ensures length (create_bc i) >= 0)
+  = match i with
+    | 0 -> ()
+    | _ -> length_create_bc_is_positive (i - 1)
+
+let rec length_create_bc_is_i (i:nat) :
+   Lemma (ensures (length (create_bc i) = i)) =
+   match i with 
+     | 0 -> ()
+     | _ -> length_create_bc_is_i (i - 1)
+
+let rec index_n_bc_is_minusone (i:nat) :
+  Lemma (ensures 
+        (let l = (create_bc i) in 
+         forall (n:nat). n < length l ==> index l n = -1))
+  = match i with
+    | 0 -> ()
+    | _ -> index_n_bc_is_minusone (i - 1)
+
 let bc : list int = create_bc alphabet_length
 
-val update_bc (l:list english_letters) (a:list english_letters) (b:list int) (i:int) : list int
-let rec update_bc l a b i = 
-    match l with 
-        | [] -> b
-        | hd::tl -> update_bc tl a (change_element_in_bc_list b 0 (alphabet_character_index hd a 0) i) (i + 1)
-        
-let final_bc : list int = update_bc pattern alphabet bc 0
+let bc_length_is_positive = length_create_bc_is_positive alphabet_length
+let bc_length_is_alphabet = length_create_bc_is_i alphabet_length
+let bc_nth_element_is_minusone = index_n_bc_is_minusone alphabet_length
 
-(*let main() =*)
-(*    let result = Printf.sprintf "Hello"*)
-(*    in *)
-(*    FStar.IO.print_string result*)
-(*    *)
-(*let _ = main()*)
+val item_index (#a:eqtype) (item:a) (l:list a) (i:nat): list nat
+let rec item_index item l i
+  = match l with 
+      | [] -> []
+      | hd::tl -> if hd = item
+                  then i :: item_index item tl (i + 1)
+                  else item_index item tl (i + 1)
 
+let item_list_length_is_zero_if_the_list_length_is_zero (#a:eqtype) (l:list a)
+  : Lemma (requires l = [])
+          (ensures forall (item:a). length (item_index item l 0) = 0)
+  = ()
+
+let item_head (#a:eqtype) (l:list a)
+  : Lemma (requires length l >= 1)
+          (ensures forall (item:a). length (item_index item [hd l] 0) <= 1)
+  = ()
+
+let rec item_head_not_equal (#a:eqtype) (l:list a)
+  : Lemma (requires length l >= 1)
+          (ensures forall (item:a). hd l <> item ==> length (item_index item [hd l] 0) = 0)
+  = match l with
+    | last -> ()
+    | hd :: tl -> item_head_not_equal tl
+
+let rec item_head_equal (#a:eqtype) (l:list a)
+  : Lemma (requires length l >= 1)
+          (ensures forall (item:a). hd l = item ==> length (item_index item [hd l] 0) = 1)
+  = match l with
+    | last -> ()
+    | hd :: tl -> item_head_equal tl
+
+let rec item_head_count (#a:eqtype) (l:list a)
+  : Lemma (requires length l >= 1) 
+          (ensures forall (item:a). length (item_index item [hd l] 0) = count item [hd l])
+  = match l with 
+    | last -> ()
+    | hd :: tl -> item_head_count tl
+
+let item_empty_list_count (a:eqtype)
+  : Lemma (ensures forall (item:a). length (item_index item [] 0) = count item [])
+  = ()
+
+let rec item_tail_count (#a:eqtype) (l:list a)
+  : Lemma (requires length l >= 1) 
+          (ensures forall (item:a). length (item_index item (tl l) 0) = count item (tl l))
+  = match l with 
+    | last -> admit()
+    | hd :: tl -> admit(item_tail_count tl)
+
+let rec item_tail (#a:eqtype) (l:list a)
+  : Lemma (requires length l >= 1)
+          (ensures forall (item:a). length (item_index item l 0) = length (item_index item [hd l] 0) + length (item_index item (tl l) 1))
+  = match l with 
+    | final -> ()
+    | hd :: tl -> item_tail tl
+
+let rec count_tail (#a:eqtype) (l:list a)
+  : Lemma (requires length l >= 1)
+          (ensures forall (item:a). count item l = count item [hd l] + count item (tl l))
+  = match l with
+    | final -> ()
+    | hd :: tl -> count_tail tl
+
+let rec item_list_has_correct_length (#a:eqtype) (l:list a)
+  : Lemma (ensures forall (item:a). length (item_index item l 0) = count item l)
+  = match l with 
+    | [] -> ()
+    | hd :: tl -> item_list_has_correct_length tl
+
+let rec item_index_is_empty (#a:eqtype) (l:list a)
+  : Lemma (ensures forall (item:a). (l = []) \/ (forall (i:nat{i < length l}). index l i <> item) ==> item_index item l 0 = [])
+  = match l with
+    | [] -> ()
+    | hd :: tl -> admit(item_index_is_empty tl)
+
+// let rec reunite_the_list (#a:eqtype) (l:list a)
+//   : Lemma (requires length l >= 1)
+//           (ensures l = append [hd l] (tl l))
+//   = match l with 
+//     | final -> ()
+//     | hd :: tl -> reunite_the_list tl
+
+let rec item_tail_not_equal (#a:eqtype) (l:list a)
+  : Lemma (requires length l >= 1)
+          (ensures forall (item:a). item_index item l 0 = append (item_index item [hd l] 0) (item_index item (tl l) 1))
+  = match l with
+    | final -> ()
+    | hd :: tl -> item_tail_not_equal tl
+
+let rec item_list_has_length_at_least_zero (#a:eqtype) (l:list a) 
+  : Lemma (ensures forall (item:a). length (item_index item l 0) >= 0)
+  = match l with
+    | [] -> ()
+    | hd :: tl -> item_list_has_length_at_least_zero tl
+
+let rec item_has_at_most_length_l_occurrences (#a:eqtype) (l:list a)
+  : Lemma (ensures forall (item:a). count item l <= length l)
+  = match l with 
+    | [] -> ()
+    | hd :: tl -> item_has_at_most_length_l_occurrences tl
+
+//correct store of indexes
+
+let rec exists_item_zero_then_correct_index (#a:eqtype) (l:list a)
+  : Lemma (requires length l > 0)
+          (ensures forall (item:a).  index l 0 = item ==> mem 0 (item_index item l 0))
+  = match l with
+    | [last] -> ()
+    | hd :: tl -> exists_item_zero_then_correct_index tl
+
+let rec exists_item_one_then_correct_index (#a:eqtype) (l:list a)
+  : Lemma (requires length l > 1)
+          (ensures forall (item:a).  index l 1 = item ==> mem 1 (item_index item l 0))
+  = match length l with
+    | 2 -> ()
+    | _ -> exists_item_one_then_correct_index (tl l)
+
+let rec exists_item_i_then_correct_index (#a:eqtype) (l:list a) (i:nat)
+  : Lemma (requires length l > i)
+          (ensures forall (item:a). index l i = item ==> mem i (item_index item l 0))
+  = let j = i + 1 in
+    match length l with
+    | j -> admit()
+    | _ -> exists_item_i_then_correct_index (tl l) i
+
+let rec index_is_or_is_not_item_is_or_is_not_mem (#a:eqtype) (l:list a)
+  : Lemma (ensures forall (item:a). forall (i:nat{i < length l}). (index l i = item || index l i <> item) ==> (mem i (item_index item l 0) = true || mem i (item_index item l 0) = false))
+  = match l with
+    | [] -> ()
+    | hd :: tl -> index_is_or_is_not_item_is_or_is_not_mem tl
+
+let rec index_is_not_item_is_not_mem (#a:eqtype) (l:list a)
+  : Lemma (ensures forall (item:a). forall (i:nat{i < length l}). index l i <> item ==> mem i (item_index item l 0) = false)
+  = match l with
+    | [] -> ()
+    | hd :: tl -> admit(index_is_not_item_is_not_mem tl)
+
+let rec exists_item_then_correct_index (#a:eqtype) (l:list a)
+  : Lemma (ensures forall (item:a). forall (i:nat{i < length l}). index l i = item ==> mem i (item_index item l 0))
+  = match l with
+    | [] -> ()
+    | hd :: tl -> admit(exists_item_then_correct_index tl)
+
+let rec correct_index_then_exists_item (#a:eqtype) (l:list a)
+  : Lemma (ensures forall (item:a). forall (i:nat{i < length l}). mem i (item_index item l 0) ==> index l i = item)
+  = match l with
+    | [] -> ()
+    | hd :: tl -> admit(correct_index_then_exists_item tl)
+
+let rec exists_item_index_iff_correct_index (#a:eqtype) (l:list a)
+  : Lemma (ensures forall (item:a). forall (i:nat{i < length l}). index l i = item <==> mem i (item_index item l 0))
+  = match l with
+    | [] -> ()
+    | hd :: tl -> exists_item_index_iff_correct_index tl;
+                  exists_item_then_correct_index l;
+                  correct_index_then_exists_item l
+
+let rec index_is_in_interval (#a:eqtype) (l:list a)
+  : Lemma (ensures forall (item:a). forall (i:nat). mem i (item_index item l 0) = true ==> i >= 0 && i < length l)
+  = match l with 
+    | [] -> ()
+    | hd :: tl -> admit(index_is_in_interval tl)
+
+let rec last_is_in_interval (#a:eqtype) (l:list a)
+  : Lemma (ensures forall (item:a). item_index item l 0 <> [] ==> last (item_index item l 0) >= 0 && last (item_index item l 0) < length l)
+  = match l with
+    | [] -> ()
+    | hd :: tl -> admit(last_is_in_interval tl)
+
+let new_or_old (#a:eqtype) (c:a) (l:list a) : int
+  = if item_index c l 0 <> []
+    then last (item_index c l 0)
+    else -1
+
+let rec not_new_or_old_empty_list (#a:eqtype) (l:list a) 
+  : Lemma (ensures forall (item:a). new_or_old item l = -1 ==> item_index item l 0 = [])
+  = match l with
+    | [] -> ()
+    | hd :: tl -> not_new_or_old_empty_list tl 
+
+let rec empty_list_length_zero (#a:eqtype) (l:list a) 
+  : Lemma (ensures forall (item:a). item_index item l 0 = [] ==> length (item_index item l 0) = 0)
+  = match l with 
+    | [] -> ()
+    | hd :: tl -> empty_list_length_zero tl
+
+//make the lemma without admit
+let rec length_zero_count_zero (#a:eqtype) (l:list a)
+  : Lemma (ensures forall (item:a). length (item_index item l 0) = 0 ==> count item l = 0)
+  = match l with
+    | [] -> ()
+    | hd :: tl -> length_zero_count_zero tl;
+                  item_list_has_correct_length l
+
+let rec count_zero_mem_false (#a:eqtype) (l:list a)
+  : Lemma (ensures forall (item:a). count item l = 0 ==> mem item l = false)
+  = match l with
+    | [] -> ()
+    | hd :: tl -> count_zero_mem_false tl
+                 
+let rec mem_false_not_item (#a:eqtype) (l:list a)
+  : Lemma (ensures forall (item:a). mem item l = false ==> (forall (i:nat). i < length l ==> index l i <> item))
+  = match l with 
+    | [] -> ()
+    | hd :: tl -> mem_false_not_item tl
+
+let rec new_or_old_not_item (#a:eqtype) (l:list a)
+  : Lemma (ensures forall (item:a). new_or_old item l = -1 ==> (forall (i:nat). i < length l ==> index l i <> item))
+  = match l with
+    | [] -> ()
+    | hd :: tl -> new_or_old_not_item tl;
+                  not_new_or_old_empty_list l;
+                  empty_list_length_zero l;
+                  length_zero_count_zero l;
+                  count_zero_mem_false l;
+                  mem_false_not_item l
+
+let rec new_or_old_not_empty_list (#a:eqtype) (l:list a)
+  : Lemma (ensures forall (item:a). new_or_old item l <> -1 ==> item_index item l 0 <> [])
+  = match l with
+    | [] -> ()
+    | hd :: tl -> new_or_old_not_empty_list tl
+
+let rec not_empty_list_length_greater_than_zero (#a:eqtype) (l:list a)
+  : Lemma (ensures forall (item:a). (item_index item l 0 <> [] && last (item_index item l 0) < length l) ==> last (item_index item l 0) >= 0)
+  = match l with
+    | [] -> ()
+    | hd :: tl -> not_empty_list_length_greater_than_zero tl                  
+
+let rec last_list_mem (#a:eqtype) (l:list a)
+  : Lemma (requires length l > 0)
+          (ensures mem (last l) l = true)
+  = match l with
+    | [hd] -> ()
+    | hd :: tl -> last_list_mem tl
+
+let length_greater_than_zero_mem (#a:eqtype) (l:list a) (item:a)
+  : Lemma (requires item_index item l 0 <> [])
+          (ensures last (item_index item l 0) >= 0 ==> mem (last (item_index item l 0)) (item_index item l 0) = true)
+  = last_list_mem (item_index item l 0)
+
+let mem_index_is_item (#a:eqtype) (l:list a) (item:a)
+  : Lemma (requires item_index item l 0 <> [] && last (item_index item l 0) < length l)
+          (ensures mem (last (item_index item l 0)) (item_index item l 0) = true ==> index l (last (item_index item l 0)) = item)
+  = exists_item_index_iff_correct_index l;
+    ()
+
+let new_or_old_not_empty_list_correct_item (#a:eqtype) (l:list a) (item:a)
+  : Lemma (requires item_index item l 0 <> [] && last (item_index item l 0) < length l)
+          (ensures new_or_old item l <> -1 ==> index l (last (item_index item l 0)) = item)
+  = new_or_old_not_empty_list l;
+    not_empty_list_length_greater_than_zero l;
+    length_greater_than_zero_mem l item;
+    mem_index_is_item l item;
+    ()
+
+val update_bc (a:list english_letters) : list int
+let rec update_bc a = 
+    match a with 
+        | [] -> []
+        | hd::tl -> (new_or_old hd pattern) :: update_bc tl
+
+let final_bc : list int = update_bc alphabet
+
+let rec final_bc_length_is_alphabet_length (a:list english_letters)
+  : Lemma (ensures length (update_bc a) = length a)
+  = match a with
+      | [] -> ()
+      | hd :: tl -> final_bc_length_is_alphabet_length tl
+
+// let rec element_not_minusone_is_part_of_the_pattern (i:nat{i < length final_bc})
+//   : Lemma (requires i < length alphabet)
+//           (ensures index final_bc i <> -1 ==> item_index (index alphabet i) (rev pattern) 0 <> -1)
+//   = match i with 
+//       | 0 -> ()
+//       | _ -> element_not_minusone_is_part_of_the_pattern (i - 1)
+
+// let rec element_not_minusone_is_in_interval (i:nat{i < length final_bc})
+//   : Lemma (ensures index final_bc i <> -1 ==> index final_bc i >= 0 && index final_bc i < length pattern)
+//   = match i with 
+//       | 0 -> ()
+//       | _ -> final_bc_length_is_alphabet_length alphabet;
+//              pattern_elements_are_in_interval 0 (index alphabet i);
+//              element_not_minusone_is_in_interval (i - 1)
+
+// let rec last_index_of_character_versus_the_next_character (i:nat) 
+//   : Lemma (requires i < length final_bc) 
+//           (ensures (index final_bc i <> -1 && i + 1 < length pattern) ==> index pattern (i + 1) <> index alphabet i)
+//   = match i with
+//       | 0 -> ()
+//       | _ -> last_index_of_character_versus_the_next_character (i - 1)
+
+// let rec last_index_of_character_stored_correctly (i:nat)
+//   : Lemma (requires i < length final_bc)
+//           (ensures index final_bc i <> -1 ==> (forall j. j > i && j < length final_bc ==> index pattern j <> index alphabet i))
+//   = match i with
+//       | 0 -> ()
+//       | _ -> last_index_of_character_stored_correctly (i - 1) 
+
+//good suffix part
 val first_characters (l:list english_letters) (j:nat{j >= 0}) : list english_letters
 let rec first_characters l j =
     match l with
@@ -99,55 +403,33 @@ let rec first_characters l j =
                       then hd :: first_characters tl (j - 1)
                       else first_characters tl j
                     
-val last_characters (l:list english_letters) (i:nat) (j:nat{j >= 0}) : list english_letters
-let rec last_characters l i j =
+val last_characters (l:list english_letters) (dim:nat) (i:nat) (j:nat{j >= 0}) : list english_letters
+let rec last_characters l dim i j =
     match l with
         | [] -> []
-        | hd::tl -> if i >= j
-                    then hd :: last_characters tl (i + 1) j
-                    else last_characters tl (i + 1) j
+        | hd::tl -> if i >= dim - j
+                    then hd :: last_characters tl dim (i + 1) j
+                    else last_characters tl dim (i + 1) j
 
-val compare_frontier (l:list english_letters) (i:nat) (j:nat{j >= 0}) : bool
-let compare_frontier l i j =
-    if first_characters l j = last_characters l i j
+val compare_frontier (l:list english_letters) (dim:nat) (i:nat) (j:nat{j >= 0}) : bool
+let compare_frontier l dim i j =
+    if first_characters l j = last_characters l dim i j && j < (length l)
     then true
     else false
     
-val maximum_frontier (l:list english_letters) (i:nat) (j:nat{j >= 0}) (k:nat) : nat
-let rec maximum_frontier l i j k =
-    let nr = length l in
+val maximum (m:int) (n:int) : int
+let maximum m n =
+    if m > n 
+    then m
+    else n
+
+val maximum_frontier (l:list english_letters) (dim:nat) (i:nat) (j:nat{j >= 0}) : nat
+let rec maximum_frontier l dim i j =
     match j with
-        | nr -> k
-        | _ -> if compare_frontier l i j = true
-               then maximum_frontier l i (j + 1) j
-               else maximum_frontier l i (j + 1) k
-
-val create_pr (l:list english_letters) (j:nat{j >= 0}) : list int
-let rec create_pr l j =
-    let nr = length l + 1 in
-    match j with 
-        | nr -> []
-        | _ -> if j = 0 
-               then (-1) :: (create_pr l (j + 1))
-               else (maximum_frontier (first_characters l j) 0 0 0) :: (create_pr l (j + 1))
-               
-let f : list int = create_pr pattern 0
-
-val give_value (f:list int) (nr:nat) (i:nat{i >= 0}) : int
-let rec give_value f nr i =
-    match f with
-        | [] -> -1
-        | hd::tl -> if i = nr
-                    then hd
-                    else give_value tl nr (i + 1)
-
-val create_gs (f:list int) (m:nat) (i:nat{i >= 0}) : list int
-let rec create_gs f m i =
-    match i with
-        | m -> []
-        | _ -> ((give_value f m 0) - m + i) :: (create_gs f m (i + 1))
-        
-let gs : list int = create_gs f (length pattern) 0
+        | 0 -> 0
+        | _ -> if compare_frontier l dim i j = true
+               then j
+               else maximum_frontier l dim i (j - 1)
 
 val append (#a:Type) (m:list a) (n:a) : list a
 let rec append m n = 
@@ -161,50 +443,95 @@ let rec reverse l =
         | [] -> []
         | hd :: tl -> append (reverse tl) hd
 
+val create_pr (l:list english_letters) (j:nat{j >= 0}) : list int
+let rec create_pr l j =
+    match j with 
+        | 0 -> [-1]
+        | _ -> (maximum_frontier (first_characters l j) (length (first_characters l j)) 0 (length (first_characters l j))) :: (create_pr l (j - 1))
+               
+let f : list int = reverse (create_pr pattern (length pattern))
+
+val give_value (f:list int) (nr:int) (i:nat{i >= 0}) : int
+let rec give_value f nr i =
+    match f with
+        | [] -> -1
+        | hd::tl -> if i = nr
+                    then hd
+                    else give_value tl nr (i + 1)
+
+val create_gs (f:list int) (m:nat) (i:nat{i >= 0}) : list int
+let rec create_gs f m i =
+    match i with
+        | 0 -> [(give_value f m 0) - m]
+        | _ -> ((give_value f m 0) - m + i) :: (create_gs f m (i - 1))
+        
+let gs : list int = reverse (create_gs f (length pattern) ((length pattern) - 1))
+ 
 let r : list english_letters = reverse pattern
-let g : list int = create_pr r 0
+let g : list int = reverse (create_pr r (length r)) 
 let h : list int = reverse g
 
 val change_value (l:list int) (m:int) (n:int) (i:nat{i >= 0}) : list int
-let rec change_value l m n i =
+let rec change_value l m n i : Tot (list int) (decreases l) =
     match l with
         | [] -> []
         | hd :: tl -> if i = m
                       then n :: change_value tl m n (i + 1)
                       else hd :: change_value tl m n (i + 1)
                       
-val update_gs (gs:list int) (h:list int) (i:nat{i >= 0}) (new_gs:list int) : list int
-let rec update_gs gs h i new_gs =
-    let nr = length gs in
-    match gs with
-        | [] -> new_gs
-        | hd :: tl -> update_gs tl h (i + 1) (change_value gs (nr - (give_value h i 0)) i 0)
+val update_gs (gs:list int) (h:list int) (i:int{i >= 0}) (dim:nat) : Tot (list int) (decreases i)
+let rec update_gs gs h i dim =
+    match i with
+        | 0 -> gs
+        | _ -> update_gs (change_value gs (dim - (give_value h (dim - i) 0)) (dim - i) 0) h (i - 1) dim
 
-let final_gs : list int = update_gs gs h 0 []
+let final_gs : list int = append (update_gs gs h (length pattern) (length pattern)) ((length pattern) - 1)
 
-val give_value_letter (f:list english_letters) (nr:nat) (i:nat{i >= 0}) : english_letters
+val give_value_letter (f:list english_letters) (nr:int) (i:nat{i >= 0}) : english_letters
 let rec give_value_letter f nr i =
     match f with
         | [] -> A
         | hd::tl -> if i = nr
                     then hd
                     else give_value_letter tl nr (i + 1)
-                  
-val maximum (m:int) (n:int) : int
-let maximum m n =
-    if m > n 
-    then m
-    else n
                     
-val boyer_moore (k:nat) (i:nat) (m:nat) (n:nat) (t:list english_letters) (p:list english_letters) (bc:list int) (gs:list int) (alphabet:list english_letters) : bool
-let rec boyer_moore k i m n t p bc gs alphabet =
-    let limit = n - m + 1 in
-    match k, i with 
-        | _, limit -> false
-        | m, _ -> true
-        | _, _ -> if give_value_letter t (i + m - 1 - k) 0 = give_value_letter p (m - 1 -k) 0
-                  then boyer_moore (k + 1) i m n t p bc gs alphabet
-                  else 
-                      let shiftbc = m - k - 1 - (give_value bc (alphabet_character_index (give_value_letter t (i + m - 1 - k) 0) alphabet 0) 0) in
-                      let shiftgs = m - k - (give_value gs (m - k) 0) in
-                      boyer_moore 0 (i + (maximum shiftbc shiftgs)) m n t p bc gs alphabet
+// val boyer_moore (k:nat) (i:nat) (m:nat) (n:nat) (t:list english_letters) (p:list english_letters) (bc:list int) (gs:list int) (alphabet:list english_letters) : Tot bool (decreases %[i;k])
+// let rec boyer_moore k i m n t p bc gs alphabet =
+//     match k, i with 
+//         | _, 0 -> false
+//         | 0, _ -> true
+//         | _, _ -> if give_value_letter t ((n - m + 1 - i) + m - 1 - (m - k)) 0 <> give_value_letter p (m - 1 - (m - k)) 0
+//                   then let shiftbc = m - (m - k) - 1 - (give_value bc (alphabet_character_index (give_value_letter t ((n - m + 1 - i) + m - 1 - (m - k)) 0) alphabet 0) 0) in
+//                        let shiftgs = m - (m - k) - (give_value gs (m - (m - k)) 0) in
+//                        let index = i - (maximum shiftbc shiftgs) in
+//                        if index >= 0 && index < i
+//                        then boyer_moore m index m n t p bc gs alphabet
+//                        else boyer_moore m 0 m n t p bc gs alphabet
+//                   else boyer_moore (k - 1) i m n t p bc gs alphabet
+
+//conversion functions, print and main
+let convert_to_int f =
+  match f with
+    | false -> 0
+    | true -> 1
+
+let string_of_int_list l =
+  Printf.sprintf "[%s]" (String.concat "; " (List.Tot.map (Printf.sprintf "%d") l))
+
+// let rec convert_letters_to_int (l:list english_letters) : list int =
+//   match l with
+//     | [] -> []
+//     | hd::tl -> (alphabet_character_index hd alphabet 0)::(convert_letters_to_int tl)
+
+// let convert_letter_to_int c =
+//   alphabet_character_index c alphabet 0
+
+let main() =
+  let message =
+     sprintf "The result is %d\n" (new_or_old J (rev pattern))
+  in
+  print_string message
+
+#push-options "--warn_error -272"
+let _ = main()
+#pop-options
